Update

regexp.v
@@ -310,11 +310,10 @@ Inductive regular : language -> Prop :=
   (* The empty language is regular *)
 | REmpty : regular lang0
 | RVoid : regular lang1
-| RAtom x A of (In x A): regular (langA x)
+| RAtom x (*x A of (In x A)*): regular (langA x)
 | RUnion L G of regular L & regular G: regular (langU L G)
 | RConcat L G of regular L & regular G: regular (langS L G)
 | RKleene G of regular G: regular (langK G)
-(*I hope this is right*)
 
 
 (* TODO: to be completed *)
@@ -381,7 +380,6 @@ Inductive regexp : Type :=
 | RE_Disjunction : regexp -> regexp -> regexp
 | RE_Concat  : regexp -> regexp -> regexp
 | RE_Kleene  : regexp -> regexp
-  (* TO BE COMPLETED *)
 .
 
 Implicit Types (r : regexp).
@@ -414,7 +412,11 @@ Fixpoint interp (r : regexp) {struct r} : language :=
 (*     regular language:                                                *)
 
 Lemma regular_regexp r : regular (interp r).
-Proof. case r. simpl. apply REmpty. simpl. apply RVoid. simpl. 
+Proof. induction r. apply REmpty. apply RVoid. apply RAtom. apply RUnion. done. done.
+apply RConcat. done. done. apply RKleene. done.
+Qed.
+
+(*case r. simpl. apply REmpty. simpl. apply RVoid. simpl. 
 
 unfold langA. todo.
 
@@ -449,15 +451,41 @@ induction r0. apply REmpty. apply RVoid. todo.
 simpl. apply RUnion. trivial. trivial.
 simpl. apply RConcat. trivial. trivial.
 simpl. apply RKleene. trivial.
-Qed.
-(*Easier way ?*)
-
+Qed.*)
 
 (* Q9. show that any regular language can be interpreted as a           *)
 (*     regular expression:                                              *)
 
+Lemma trans (L G H: language): L =L G -> G =L H -> L =L H.
+Proof. unfold eqL. move => LG GH. move => w. rewrite LG. rewrite GH. reflexivity.
+Qed.
+
+Lemma interpUnion (L1 L2 G1 G2: language): L1 =L L2 -> G1 =L G2 -> langU L1 G1 =L langU L2 G2.
+Proof. unfold eqL. move => L12 G12. unfold langU. move => w. rewrite L12. rewrite G12. reflexivity.
+Qed.
+
+Lemma interpConcat (L1 L2 G1 G2: language): L1 =L L2 -> G1 =L G2 -> langS L1 G1 =L langS L2 G2.
+Proof. unfold eqL. move => L12 G12. unfold langS. move => w. split. move => h. 
+destruct h. destruct H. destruct H. destruct H0. exists x. exists x0. rewrite H. split. trivial.
+split. apply L12. trivial. apply G12. trivial.
+move => h. destruct h. destruct H. destruct H. destruct H0. exists x. exists x0. rewrite H. split. trivial.
+split. apply L12. trivial. apply G12. trivial.
+Qed.
+
+Lemma interpKleene (L G: language): L =L G -> langK L =L langK G.
+Proof. unfold eqL. move => LG. move => w. induction w. split. move => Lnil. apply langK_nil.
+move => Gnil. apply langK_nil.
+Admitted.
+
 Lemma regexp_regular L : regular L -> exists r, L =L interp r.
-Proof. move => regL. unfold eqL. todo. Qed.
+Proof. move => rL. induction rL. destruct IHrL. exists x. move: H H0. apply trans.
+exists RE_Empty. simpl. done.
+exists RE_Void. simpl. done.
+exists (RE_Atom x). simpl. done.
+destruct IHrL1. destruct IHrL2. exists (RE_Disjunction x x0). simpl. apply interpUnion. trivial. trivial.
+destruct IHrL1. destruct IHrL2. exists (RE_Concat x x0). simpl. apply interpConcat. trivial. trivial.
+destruct IHrL. exists (RE_Kleene x). simpl. apply interpKleene. trivial.
+Qed.
 
 (* Of course, it may happen that two regular expressions represent      *)
 (* the same language: r1 ~ r2 iff [r1] = [r2].                          *)
@@ -466,7 +494,7 @@ Proof. move => regL. unfold eqL. todo. Qed.
 (*      eqR r1 r2 iff r1 and r2 are equivalent regexp.                  *)
 
 Definition eqR (r1 r2 : regexp) : Prop := 
-  forall w, (interp r1) w <-> (interp r2) w.
+  eqL (interp r1) (interp r2).
 
 Infix "~" := eqR (at level 90).
 
@@ -509,8 +537,8 @@ Fixpoint contains0 (r : regexp) : bool :=
   | RE_Void  => true
   | RE_Atom A => false
   | RE_Disjunction r1 r2 => contains0 r1 || contains0 r2
-  | RE_Concat r1 r2 => contains0 r1 || contains0 r2
-  | RE_Kleene regexp => contains0 regexp
+  | RE_Concat r1 r2 => contains0 r1 && contains0 r2
+  | RE_Kleene regexp => true (* not contains0 regexp*)
   end.
   
 
@@ -520,18 +548,19 @@ Lemma contains0_ok r : contains0 r <-> interp r nil.
 Proof. induction r. 
 
 simpl. unfold lang0. split. auto. auto.
-
 simpl. unfold lang1. split. auto. auto.
-
-simpl. unfold langA. todo.
-
-simpl. todo.
-
-simpl. todo.
-
-simpl. todo.
-
- Qed.
+simpl. done.
+simpl. unfold langU. split. move => cont. case a: (contains0 r1). left. apply IHr1. apply a.
+right. apply IHr2. move: cont. rewrite a. simpl. trivial.
+case a: (contains0 r1). done. simpl. case. move => b. apply IHr1 in b. move: b. rewrite a. done. apply IHr2.
+simpl. unfold langS. split. move => cont. exists nil. exists nil. split. trivial. split.
+apply IHr1. case a: (contains0 r1). trivial. move: cont. rewrite a. simpl. trivial.
+apply IHr2. case a: (contains0 r2). trivial. move: cont.  rewrite a. simpl. apply Bool.andb_true_iff.
+move => whole. destruct whole. destruct H. destruct H. destruct H0. apply app_eq_nil in H. destruct H.
+rewrite H in H0. apply IHr1 in H0. rewrite H2 in H1. apply IHr2 in H1. apply Bool.andb_true_iff. done.
+simpl. split. move => cont. apply langK_nil.
+trivial.
+Qed.
 
 (* We give below the definition of the Brzozowski's derivative:         *)
 (*                                                                      *)
@@ -564,7 +593,7 @@ Fixpoint Brzozowski (x : A) (r : regexp) : regexp :=
   | RE_Atom A => if (Aeq x A) then RE_Void else RE_Empty
   | RE_Disjunction r1 r2 => RE_Disjunction (Brzozowski x r1) (Brzozowski x r2)
   | RE_Concat r1 r2 => RE_Disjunction (RE_Concat (Brzozowski x r1) r2) (RE_Concat (if contains0 r1 then RE_Void else RE_Empty) (Brzozowski x r2))
-  | RE_Kleene regexp => (Brzozowski x regexp)
+  | RE_Kleene regexp => RE_Concat (Brzozowski x regexp) (RE_Kleene regexp)
   end.
   
   
@@ -572,41 +601,37 @@ Fixpoint Brzozowski (x : A) (r : regexp) : regexp :=
 (* Q15. write a function `rmatch` s.t. `rmatch r w` checks wether a     *)
 (*      word `w` matches a given regular expression `r`.                *)
 
-Definition rmatch (r : regexp) (w : word) : bool := todo.
+Fixpoint rmatch (r : regexp) (w : word) : bool := 
+  match w with
+  | nil => if contains0 r then true else false
+  | a :: wr => rmatch (Brzozowski a r) wr
+  end.
 
 (* Q16. show that the `Brzozowski` function is correct.                 *)
 
 Lemma Brzozowski_correct (x : A) (w : word) (r : regexp) :
   interp (Brzozowski x r) w -> interp r (x :: w).
-Proof. case r. simpl. unfold lang0. trivial. simpl. unfold lang0. unfold lang1. move => fls. case fls. 
+Proof. induction r. simpl. unfold lang0. trivial.
+simpl. unfold lang0. done.
+simpl. case dec: Aeq. apply Aeq_dec in dec. simpl. unfold lang1. move => wnil. unfold langA. rewrite dec.
+rewrite wnil. reflexivity.
+simpl. unfold lang0. done.
+simpl. unfold langU. case. move => a. left. move: a. apply IHr1.
+move => a. right. move: a. apply IHr2.
+simpl. unfold langU. unfold langS.
 
-todo.
+todo. 
 
-simpl. induction r0. simpl. unfold langU. move => r0. case. unfold lang0. case. unfold lang0.
-induction r0. simpl. unfold lang0. case. simpl. unfold lang0. case.
+todo. 
 
-simpl. case Aeq. simpl. unfold lang1. move => wnil. rewrite wnil. right. unfold langA. todo.
-
-simpl. unfold lang0. case.
-
-simpl. unfold langU. case. 
-move => h. move: (IHr0_1 h). case. case. move => a. right. left. apply a.
-move => h. move: (IHr0_2 h). case. case. move => a. right. right. apply a.
-
-todo. (*simpl. unfold langS. unfold langU. case.*)
-
-simpl. move => h. right. move: (IHr0 h). case. case. (*huh?*)todo.
-
-todo. todo. todo. todo. todo. todo. todo.
-
-(*this will take forever*)
 Qed.
 
 (* Q17. show that `rmatch` is correct.                                  *)
 
-Lemma rmatch_correct (r : regexp) (w : word):
-  rmatch r w -> interp r w.
-Proof. todo. Qed.
+Lemma rmatch_correct (r : regexp) (w : word): rmatch r w -> interp r w.
+Proof. move: r. induction w. simpl. move => r. case cont: (contains0 r). move => true. apply contains0_ok. apply cont. done.
+simpl. move => r rm. apply Brzozowski_correct. move: rm. apply IHw.
+Qed.
 
 (* Q18. (HARD - OPTIONAL) show that `rmatch` is complete.               
 
